\begin{enumerate}[label=\thesection.\arabic*.,ref=\thesection.\theenumi]
\numberwithin{equation}{enumi}

\item Fig. \label{fig:ee18btech11019_hart} shows a Hartley oscillator.

\begin{figure}[ht]
    \begin{center}
	    \resizebox{\columnwidth}{!}{\input{./figs/hart.tex}}
	\end{center}
\caption{Hartley oscillator}
\label{fig:ee18btech11019_hart}
\end{figure}
\item Draw the equivalent block diagram of an oscillator.\\
\solution
\begin{figure}[!ht]
    \begin{center}
		
		\resizebox{\columnwidth}{!}{\input{./figs/osc.tex}} %block diagram
	\end{center}
\caption{block diagram for oscillator}
\label{fig:ee18btech11019_hart_block}
\end{figure}
Fig. \label{fig:ee18btech11019_hart_block} shows the block diagram of the an Oscillator in Fig. \ref{fig:ee18btech11019_hart_block}.\\




\item Show that the gain of the oscillator is \\
\begin{align}
    Gain  = \frac{V_{out}}{V_{in}} = \frac{G}{1 - GH}
\label{eq:ee18btech11019_gain}
\end{align}
%
\\
\solution From figure \ref{fig:ee18btech11019_hart_block}
Oscillators gain can be given as follows:\\
\begin{align}
    G(V_{in} + HV_{out}) =V_{out}\\
    G(V_{in} = (1-GH)V_{out}\\
    \frac{V_{out}}{V_{in}} = \frac{G}{1 - GH}
\end{align}
%
resulting in \eqref{eq:ee18btech11019_gain}.\\



\item State the condition for sustained oscillations. Justify.

\solution Condition for sustained oscillation is given by\\
\begin{align}
    GH = 1
\end{align}
Along with, total phase gain o the circuit should be 0 or 2$\pi$\\
\textbf{Justification:} as, when $ GH =1 $, gain becomes infinity, and theoretically we can get output, without actually providing input\\
Total phase gain should be so, as we want our signal to be in phase after every loop traversal.\\


\item Find $G$ and $H$.

\solution From the figure \ref{fig:ee18btech11019_block3}\\

\begin{figure}[!ht]
    \begin{center}
		\resizebox{\columnwidth}{!}{\input{./figs/lc.tex}}
		
	\end{center}
\caption{Amplifier written in equivalent circuit form}
\label{fig:ee18btech11019_block3}
\end{figure}
W.K.T, no current flows in the opamp terminals.\\
and,(in S-domain)\\
\begin{align}
    A(V_1 - V_2) = V_{out}\\
    v_2 =0\\
    V_1 = V_{out} + iR_2
\end{align}
where,\\
A is the gain through the amplifier,\\
Assuming everything at 0 initially.\\
\begin{align}
    V_{out} - i_1SL_1 = 0\\
    i_1(SL_1 + SL_2) = i_2(\frac{1}{SC})
\end{align}
On solving\\
\begin{align}
    i_1 = \frac{V_{out}}{SL_1}\\
    i_2 = ((SL_1 + SL_2)SC)(\frac{V_{out}}{SL_1})\\
\end{align}
Now,\\
\begin{align}
    i = i_1 + i_2\\
    i = ((SL_1 + SL_2)SC + 1)\frac{V_{out}}{SL_1}\\
\end{align}
Finding $V_1$
\begin{align}
    V_1 = V_{out} + iR_2 \\
                = V_{out} ( 1 + R_2\frac{((SL_1 + SL_2)SC + 1)}{SL_1})\\
\end{align}
Gain, G(s) is given by,
\begin{align}
G = kA\\
\therefore A = \frac{V_{out}}{V_1}\\
    = \frac{1}{1 + R_2\frac{((SL_1 + SL_2)SC + 1)}{SL_1}}
\end{align}
where, k is some real number.\\
\begin{align}
H(s) = \frac{V_{out}}{V_{f}} =\frac{ i_1SL_1}{i_1SL_2}
    = \frac{L_1}{L_2}
\label{eq:ee18btech11019_B_gain}      
\end{align}

\item Find the frequency of oscillation using the condition that $GH = 1$.

\solution 
Now,we know that $GH = 1$ for sustained oscillations, putting the the above terms in the equation\\
on solving,\\
    
putting that in and equating $GH=1$ we get,

\begin{align}
    1 = (\frac{L_1}{L_2})\frac{k}{1 + R_2\frac{((SL_1 + SL_2)SC + 1)}{SL_1}}
\end{align}

As we need, to find frequency, put S =jw
\begin{align}
   1 = (\frac{L_1}{L_2})\frac{k}{1 + R_2\frac{((j\omega L_1 + j\omega L_2)j\omega C + 1)}{j\omega L_1}}\\
   1 = (\frac{L_1}{L_2})\frac{k}{1 -j R_2\frac{(-(\omega L_1 + \omega L_2)\omega C + 1)}{\omega L_1}}\\
\end{align}
To satisfy the above equation, equating imaginary term to Zero.
\begin{align}    
    \omega L_1 + \omega L_2  = \frac{1}{\omega C}\\
    \omega = \frac{1}{\sqrt{(L_1+L_2)(C)}}\\
    f = \frac{1}{2\pi \sqrt{(L_1+L_2)(C)}}
\end{align}
Therefor, G for sustained oscillations can be given by,\\
\begin{align}
    G = \frac{1}{H}
     =  \frac{L_2}{L_1} 
\label{eq:ee18btech11019_Amp_gain}
\end{align}
 
\item For Hartley oscillator frequency generated can be given as 
\begin{align}
    f = \frac{1}{2\pi\sqrt{(L_1 + L_2)C}}
    \label{eq:ee18btech11019_frequency}
\end{align}

We know that for an opamp gain is given by:
\begin{align}
    G = \frac{R_2}{R_1}
\end{align}
Here,
\begin{align}
    G(S) = \frac{R_2}{R_1} = \frac{L_2}{L_1}
\end{align}
referring to \ref{eq:ee18btech11019_Amp_gain}\\
And,
\begin{align}
    H(s) = \frac{V_o}{V_f} = \frac{L_1}{L_2}
\end{align}
referring to \ref{eq:ee18btech11019_B_gain}\\
\newline
\item \textbf{Simulation:}\\
Taking the following values,and applying in \ref{eq:ee18btech11019_frequency} \\



\begin{tabular}{|c|c|}
\hline
Component & Value  \\
\hline
$R_1$         & 10K$\Omega$   \\
\hline
$R_2$         & 100K$\Omega$   \\
\hline
$R_3$         & $\sim$  \\
\hline
$L_1$         & $1 \mu H$     \\
\hline
$L_2$         & $1 \mu H$   \\
\hline
C         & 120 pF \\
\hline
\end{tabular}
\\

We get f = 103 MHz\\
Feedback factor for Hartley given by:
\begin{align}
H =\frac{L_1}{L_2}= 1
\end{align}
W.K.T, $GH = 1$, for sustained oscillation \\
$\therefore$ Minimum amplification Gain,G = 1\\ (GH <=1 for a stable system) \\
\end{enumerate}
